

The RHS of the previous equation is clearly nonpositive, so α' must be nonpositive as well. We can also bound the size of α' with

$$\begin{aligned} -\varepsilon\alpha' &= \left\lceil \frac{\alpha}{1+\varepsilon} \right\rceil - \alpha \\ 1 - \varepsilon\alpha' &\geq 1 + \frac{\alpha}{1+\varepsilon} - \alpha \\ -\varepsilon\alpha' &\geq \frac{-\varepsilon\alpha}{1+\varepsilon} \\ (1+\varepsilon)\alpha' &\leq \alpha \\ \alpha' &< \alpha. \end{aligned}$$

By (1), if we take the lower bound for the change in $\sum E_k^2$ using α' , the value of $\sum E_{k-1}^2$ is equal to or smaller than if we had used α instead. By the same logic that was used to prove Lemma 13, it is always helpful to have a lower $\sum E^2$. \square

With Lemma 13 and Lemma 14, we now have a strictly stronger set of actions on $\sum E$ and $\sum E^2$ that we can perform with each move.

Definition 15. A *strong reversed move* that uses α on the pair of values $\sum E_k$ and $\sum E_k^2$ is given by

$$\begin{aligned} \sum E_{k-1} &= \sum E_k - \varepsilon\alpha \\ \sum E_{k-1}^2 &= \sum E_k^2 - 2\sum E_k + (1-\varepsilon)^2\alpha^2. \end{aligned}$$

For integers $1 \leq k \leq m$, let α_k denote the value of α used in the strong reversed move to get from $(\sum E_k, \sum E_k^2)$ to $(\sum E_{k-1}, \sum E_{k-1}^2)$. Then,

$$\begin{aligned} \sum E_m &= \sum E_0 + \varepsilon\alpha_1 + \varepsilon\alpha_2 + \cdots + \varepsilon\alpha_m \\ \sum E_m &= \sum E_0 + \varepsilon \sum_{j=1}^m \alpha_j. \end{aligned} \tag{3}$$

The same process is a little more complicated for $\sum E_m^2$.

$$\sum E_m^2 = \sum E_0^2 + 2 \sum_{j=1}^m \left(\sum E_j \right) - (1-\varepsilon)^2 \sum_{j=1}^m \alpha_j^2$$

We can rewrite the $\sum E_j$ by plugging in (3).

$$\begin{aligned} \sum E_m^2 &= \sum E_0^2 + 2 \sum_{j=1}^m \left(\sum E_j \right) - (1-\varepsilon)^2 \sum_{j=1}^m \alpha_j^2 \\ \sum E_m^2 &= \sum E_0^2 + 2 \sum_{j=1}^m \left(\sum E_0 + \varepsilon \sum_{i=1}^j \alpha_i \right) - (1-\varepsilon)^2 \sum_{j=1}^m \alpha_j^2 \\ \sum E_m^2 &= \sum E_0^2 + 2m \sum E_0 + 2\varepsilon \sum_{j=1}^m (m-j+1)\alpha_j - (1-\varepsilon)^2 \sum_{j=1}^m \alpha_j^2 \\ 0 &= \sum E_0^2 + 2m \sum E_0 - \sum E_m^2 + 2\varepsilon \sum_{j=1}^m (m-j+1)\alpha_j - (1-\varepsilon)^2 \sum_{j=1}^m \alpha_j^2 \end{aligned}$$